RAC of arithmetic properties: include function call in example, cleanups

Playground.v
@@ -5,23 +5,19 @@ Require Import RAC.Semantics.
 Require Import ZArith.ZArith.
 Require Import String.
 From Coq Require Import Lists.List.
-From Coq Require Import Logic.FunctionalExtensionality.
 Open Scope string_scope.
-Open Scope Z_scope.
 
-
-Open Scope mini_c_scope. 
-Open Scope fsl_scope.
-
+Fact ir2 : Int.inRange 2. now split. Qed.
 Fact ir3 : Int.inRange 3. now split. Qed.
 Fact ir5 : Int.inRange 5. now split. Qed.
 Fact ir10 : Int.inRange 10 . now split. Qed.
 Fact ir14 : Int.inRange 14. now split. Qed.
 Fact ir15 : Int.inRange 15. now split. Qed.
-Definition three := Int (Int.of_z 3 ir3).
-Definition five := Int (Int.of_z 5 ir5).
-Definition ten := Int (Int.of_z 10 ir10).
-Definition fifteen := Int (Int.of_z 15 ir15).
+Definition three := Int (Int.mkMI 3 ir3).
+Definition five := Int (Int.mkMI 5 ir5).
+Definition ten := Int (Int.mkMI 10 ir10).
+Definition fifteen := Int (Int.mkMI 15 ir15).
+Definition funs := ⊥{"test"\("a" :: "b" :: nil, <{ return ("b") }>)}.
 
 
 Example stmt_test :
@@ -30,24 +26,24 @@ Example stmt_test :
     let l := snd o in 
     c_stmt_sem
     o m 
-    
+
     <{
-        "x" := 5 ;
-        "y" := 10;
-        "z" := "x" + "y";
-        "g" := 0;
+    "x" = 5 ;
+    "y" = 10;
+    "z" = "x" + "y";
+    "g" = 0;
+    "out" <-  (1+2, ("x"+"g")) "test";
 
-        if ("z" <= 14)
-            "g" := "z"
-        else 
-            "g" := "z" / 5
-
-   }>
+    if ("z" <= 14)
+        "g" = "z"
+    else 
+        "g" = "out" / 5
+    }>
     
-    (v{"g"\ three, "g"\ zero, "z"\ fifteen, "y"\ ten, "x" \ five}, l) m
+    (v{"g"\ one, "out"\five, "g"\ zero, "z"\ fifteen, "y"\ ten, "x" \ five}, l) m
    .
 Proof.
-    intros.
+    intros. 
      apply S_Seq with (v{"x" \ five},l) m.
      apply S_Assign. apply C_E_Int.
      apply S_Seq with (v{"y"\ten,"x"\five}, l) m.
@@ -57,17 +53,35 @@ Proof.
           now apply C_E_Var. 
         + apply S_Seq  with (v{"g"\ zero, "z" \ fifteen, "y" \ ten, "x" \ five}, l) m. 
           ++ apply S_Assign. apply C_E_Int.
-          ++ apply S_IfFalse with zero.
+          ++ apply S_Seq with (v{"out"\five, "g"\ zero, "z" \ fifteen, "y" \ ten, "x" \ five}, l) m.
+          {  
+          apply S_FCall with
+              (resf:="out")
+              (z:=five)
+              (env':=  (⊥{"out"\five, "b" \ five, "a" \ three}, ⊥))
+              (b := <{ return ("b") }>)
+              (funs:=funs)
+              (zargs := three::five::nil)
+              (xargs := "a"::"b"::nil)
+            .
+            - reflexivity.
+            - simpl. constructor. 
+                apply C_E_BinOpInt with  (z:=1) (z':=2) (z_ir:=oneinRange) (z'_ir:=ir2) ; now constructor.
+                constructor.
+                apply C_E_BinOpInt with  (z:=5) (z':=0) (z_ir:=ir5) (z'_ir:=zeroinRange) ; now constructor.
+                constructor.
+            - simpl. constructor. now constructor.
+            - simpl. constructor.
+            }
+           apply S_IfFalse with zero.
             * apply C_E_BinOpFalse with 15 14 ir15 ir14 ; try now constructor.
             simpl. intro H. destruct H. reflexivity.
             * reflexivity.
-            * apply S_Assign. apply C_E_BinOpInt with  (z:=15) (z':=5) (z_ir:=ir15) (z'_ir:=ir5); now constructor.
+            * apply S_Assign. apply C_E_BinOpInt with  (z:=(5)) (z':=5) (z_ir:=ir5) (z'_ir:=ir5) ; now constructor.
 Qed.
 
 
 Close Scope mini_c_scope.
 
-
-
 Example test_dom : ~ dom (fun x => if x>?2 then Some (x*2) else None) 2.
-Proof. intro contra. inversion contra. destruct H. discriminate. Qed.
+Proof. intro contra. inversion contra. discriminate. Qed.
