Semantics.v
@@ -3,29 +3,27 @@ Require Import RAC.Notations.
 Require Import RAC.Utils.
 Require Import ZArith.ZArith.
 From Coq Require Import Strings.String.
-Open Scope fsl_scope.
-Open Scope Z_scope.
 Open Scope mini_c_scope.
 
 
-Inductive c_exp_sem (env : Ω) : c_exp -> Values -> Prop :=
-| C_E_Int (z:Z) in_range: env ⊨ z => (Int.of_z z in_range)
+Inductive c_exp_sem (env : Ω) : c_exp -> Value -> Prop :=
+| C_E_Int (z:Z) in_range: env ⊨ z => (Int.mkMI z in_range)
 | C_E_Var (x:V) z  : 
     (fst env)(x:string) = Some (Int z) -> 
     env ⊨ x => z
 | C_E_BinOpInt e e' (z z':Z) op z_ir z'_ir 
     (H:Int.inRange (⋄ op z z')) :
-    env ⊨ e =>  (Int.of_z z z_ir) ->
-    env ⊨ e' =>  (Int.of_z z' z'_ir) ->
-    env ⊨ BinOpInt e op e' => Int.of_z ((⋄ op) z z') H
+    env ⊨ e =>  (Int.mkMI z z_ir) ->
+    env ⊨ e' =>  (Int.mkMI z' z'_ir) ->
+    env ⊨ BinOpInt e op e' => Int.mkMI ((⋄ op) z z') H
 | C_E_BinOpTrue e e' (z z' : Z) z_ir z'_ir op :
-    env ⊨ e => (Int.of_z z z_ir) ->
-    env ⊨ e' => (Int.of_z z z'_ir) ->
+    env ⊨ e => (Int.mkMI z z_ir) ->
+    env ⊨ e' => (Int.mkMI z z'_ir) ->
     ((◁ op) z z' -> True) ->
     env ⊨ BinOpBool e op e' => one
 | C_E_BinOpFalse e e' (z z' : Z) op z_ir z'_ir :
-    env ⊨ e => (Int.of_z z z_ir) -> 
-    env ⊨ e' => (Int.of_z z' z'_ir) -> 
+    env ⊨ e => (Int.mkMI z z_ir) -> 
+    env ⊨ e' => (Int.mkMI z' z'_ir) -> 
     ((◁ op) z z' -> False) ->
     env ⊨ BinOpBool e op e' => zero
 
@@ -33,7 +31,7 @@ where  "Ω '⊨' e => v" := (c_exp_sem Ω e v).
 
 
 Inductive c_decl_sem (env:Ω) (mem:M) : c_decl -> Ω -> M -> Prop := 
-    | Decl t x (u:Values) : 
+    | Decl t x (u:Value) : 
         (* v x = ⊥ -> (env,mem ⊨ C_Decl t x => (v{x\u},l),mem) *)
         c_decl_sem  env mem (C_Decl t x) ((fst env){x\u}, snd env) mem 
   (* where 
@@ -46,15 +44,15 @@ Inductive c_stmt_sem (env:Ω) (mem:M) : S -> Ω -> M -> Prop :=
     | S_Assign x z e : 
         (* in v x Int + Uint  *)
         env ⊨ e => z ->
-        c_stmt_sem  env mem <{x := e}> ((fst env){x\z},snd env) mem
+        c_stmt_sem  env mem <{x = e}> ((fst env){x\z},snd env) mem
     | S_IfTrue env' mem' z e s s' :
         env ⊨ e => z ->
-        z <>  Int.of_z 0 zeroinRange ->
+        z <>  Int.mkMI 0 zeroinRange ->
         c_stmt_sem env mem s  env' mem' ->
-        c_stmt_sem  env mem <{ if (e) s else s' }> env' mem' 
+        c_stmt_sem  env mem <{ if (e) s else s'}> env' mem' 
     | S_IfFalse env' mem' z e s s' :
         env ⊨ e => z ->
-        z = Int.of_z 0 zeroinRange ->
+        z = Int.mkMI 0 zeroinRange ->
         c_stmt_sem  env mem s' env' mem' ->
         c_stmt_sem  env mem <{ if (e) s else s' }> env' mem' 
     | S_While e s   env' mem' :
@@ -102,7 +100,7 @@ Inductive c_stmt_sem (env:Ω) (mem:M) : S -> Ω -> M -> Prop :=
 
 (* TODO: finish mini-fsl semantic *)
 
-Inductive fsl_term_sem (env:Ω) : LT -> Values -> Prop :=
+Inductive fsl_term_sem (env:Ω) : LT -> Value -> Prop :=
 | FSL_E_Int z : fsl_term_sem env z UMpz
 | FSL_E_LVar x z : (snd env) x = Some z -> fsl_term_sem env x UMpz
 | FSL_E_Var x v : (fst env) v = Some x ->  fsl_term_sem env v x
@@ -111,7 +109,7 @@ Inductive fsl_term_sem (env:Ω) : LT -> Values -> Prop :=
     values_int z' = Some (Int z'int) ->
     fsl_term_sem env t z ->
     fsl_term_sem env t' z' ->
-    ~ (op = FSL_Div /\ zint = (Int (Int.mkMI 0 zeroinRange))) ->
+    ~ (op = FSL_Div /\ zint = (Int (mkMI 0 zeroinRange))) ->
     fsl_term_sem env (T_BinOp t op t') ((fsl_binop_int_model op) zint z'int) *)
 .
 
@@ -122,7 +120,7 @@ Inductive fsl_term_sem (env:Ω) : LT -> Values -> Prop :=
 
 (* 
 Inductive fsl_assert_sem : S -> Ω -> M -> Ω -> M -> Prop := 
-| P_Assert env mem p :  env ⊨ p => Int.of_z 1 oneinRange -> 
+| P_Assert env mem p :  env ⊨ p => mkMI 1 oneinRange -> 
     fsl_assert_sem (LAssert p) env mem env mem
 . *)
 
