Utils.v
@@ -2,15 +2,13 @@ From RAC Require Import Notations.
 From Coq Require Import ZArith.ZArith.
 From Coq Require Import Setoids.Setoid.
 From Coq Require Import Eqdep_dec. 
-
 Open Scope Z_scope.
-Open Scope fsl_scope.
-Open Scope list_scope.
+Open Scope utils_scope.
 
 Definition partial_function {X Y : Type} := X -> option Y.
 Definition empty_p {X Y:Type} := fun (_:X) => (None: option Y).
 
-Notation "⊥" := empty_p : fsl_scope.
+Notation "⊥" := empty_p : utils_scope.
 
 Class EqDec X :=
 {
@@ -22,8 +20,7 @@ Class EqDec X :=
 Definition p_map {X Y : Type} `{EqDec X}  (f: X -> option Y) (xy:X * Y) : X -> option Y :=
     fun i => if eq_dec (fst xy) i then Some (snd xy) else f i.
 
-Notation "f { xy , .. , xy' }" :=  (p_map .. (p_map f xy') .. xy ) : fsl_scope.
-
+Notation "f { xy , .. , xy' }" :=  (p_map .. (p_map f xy') .. xy ) : utils_scope.
 
 
 Definition p_map_addall {X Y: Type} `{EqDec X} env (l:list (X*Y)) :=
@@ -31,10 +28,9 @@ Definition p_map_addall {X Y: Type} `{EqDec X} env (l:list (X*Y)) :=
 .
 
 
-Inductive domain { X Y : Type} (f: X ⇀ Y) (x:X) := 
-    | exist: (exists y, (f x) = Some y) ->  domain f x
+Definition domain { X Y : Type} (f: X ⇀ Y) (x:X) := (exists y, (f x) = Some y) 
 .
-Notation "'dom' f" := (domain f) : fsl_scope.
+Notation "'dom' f" := (domain f) : utils_scope.
 
 
 Module Type Bounds.
@@ -49,7 +45,6 @@ Module MachineInteger(B:Bounds).
     Record MI := mkMI {val : Z; in_range : inRange val}.
     
     Definition to_z (i:MI) : Z := i.(val).
-    Definition of_z (val:Z) H : MI := mkMI val H.
     Definition mi_eqb m1 m2 := val m1 =? val m2.
 End MachineInteger.
 
